
## Derivatives Rules

- **Power Rule:**  $\dfrac{d}{dx}\left(x^a\right)=a\cdot x^{a-1}$|
- **Derivative of a constant**:  $\dfrac{d}{dx}\left(a\right)=0$
- **Sum Difference Rule**:  $\left(f\pm g\right)^{'}=f^{'}\pm g^{'}$
- Constant Out $\left(a\cdot f\right)^{'}=a\cdot f^{'}$
- Product Rule $\left(f\cdot g\right)^{'}=f^{'}\cdot g+f\cdot g^{'}$
- Quotient Rule $\left(\dfrac{f}{g}\right)^{'}=\dfrac{f^{'}\cdot g-g^{'}\cdot f}{g^2}$
- Chain rule $\dfrac{df\left(u\right)}{dx}=\dfrac{df}{du}\cdot\dfrac{du}{dx}$

  
  

## Common Derivatives

- $\dfrac{d}{dx}\left(\ln\left(x\right)\right)=\dfrac{1}{x}$
- $\dfrac{d}{dx}\left(\ln\left(\left|x\right|\right)\right)=\dfrac{1}{x}$
- $\dfrac{d}{dx}\left(e^x\right)=e^x$
-  $\dfrac{d}{dx}\left(\log\left(x\right)\right)=\dfrac{1}{x\ln\left(10\right)}$
-  $\dfrac{d}{dx}\left(\log\_a\left(x\right)\right)=\dfrac{1}{x\ln\left(a\right)}$

## Trigonometric Derivatives
- $\dfrac{d}{dx}\left(\sin\left(x\right)\right)=\cos\left(x\right)$
- $\dfrac{d}{dx}\left(\cos\left(x\right)\right)=-\sin\left(x\right)$
- $\dfrac{d}{dx}\left(\tan\left(x\right)\right)=\sec^2\left(x\right)$
- $\dfrac{d}{dx}\left(\sec\left(x\right)\right)=\dfrac{\tan\left(x\right)}{\cos\left(x\right)}$
- $\dfrac{d}{dx}\left(\csc\left(x\right)\right)=\dfrac{-\cot\left(x\right)}{\sin\left(x\right)}$
-  $\dfrac{d}{dx}\left(\cot\left(x\right)\right)=-\dfrac{1}{\sin^2\left(x\right)}$ddx (cot(x))\=−1sin<sup class=""><span>2</span></sup>(x) 

  
  

## Arc Trigonometric Derivatives

$\dfrac{d}{dx}\left(\arcsin\left(x\right)\right)=\dfrac{1}{\sqrt{1-x^2}}$ddx (arcsin(x))\=1√1−x<sup class=""><span>2</span></sup>  $\dfrac{d}{dx}\left(\arccos\left(x\right)\right)=-\dfrac{1}{\sqrt{1-x^2}}$ddx (arccos(x))\=−1√1−x<sup class=""><span>2</span></sup> 

$\dfrac{d}{dx}\left(\arctan\left(x\right)\right)=\dfrac{1}{x^2+1}$ddx (arctan(x))\=1x<sup class=""><span>2</span></sup>+1  $\dfrac{d}{dx}\left(\arcsec\left(x\right)\right)=\dfrac{1}{\sqrt{x^2\left(x^2-1\right)}}$ddx (arcsec(x))\=1√x<sup class=""><span>2</span></sup>(x<sup class=""><span>2</span></sup>−1) 

$\dfrac{d}{dx}\left(\arccsc\left(x\right)\right)=-\dfrac{1}{\sqrt{x^2-1}\left|x\right|}$ddx (arccsc(x))\=−1√x<sup class=""><span>2</span></sup>−1|x|  $\dfrac{d}{dx}\left(\arccot\left(x\right)\right)=-\dfrac{1}{x^2+1}$ddx (arccot(x))\=−1x<sup class=""><span>2</span></sup>+1 

  
  

## Hyperbolic Derivatives

$\dfrac{d}{dx}\left(\sinh\left(x\right)\right)=\cosh\left(x\right)$ddx (sinh(x))\=cosh(x) $\dfrac{d}{dx}\left(\cosh\left(x\right)\right)=\sinh\left(x\right)$ddx (cosh(x))\=sinh(x)

$\dfrac{d}{dx}\left(\tanh\left(x\right)\right)=\sech^2\left(x\right)$ddx (tanh(x))\=sech<sup class=""><span>2</span></sup>(x) $\dfrac{d}{dx}\left(\sech\left(x\right)\right)=\tanh\left(x\right)\left(-\sech\left(x\right)\right)$ddx (sech(x))\=tanh(x)(−sech(x))

$\dfrac{d}{dx}\left(\csch\left(x\right)\right)=-\coth\left(x\right)\csch\left(x\right)$ddx (csch(x))\=−coth(x)csch(x) $\dfrac{d}{dx}\left(\coth\left(x\right)\right)=-\csch^2\left(x\right)$ddx (coth(x))\=−csch<sup class=""><span>2</span></sup>(x)

  
  

## Arc Hyperbolic Derivatives

$\dfrac{d}{dx}\left(\arcsinh\left(x\right)\right)=\dfrac{1}{\sqrt{x^2+1}}$ddx (arcsinh(x))\=1√x<sup class=""><span>2</span></sup>+1  $\dfrac{d}{dx}\left(\arccosh\left(x\right)\right)=\dfrac{1}{\sqrt{x-1}\sqrt{x+1}}$ddx (arccosh(x))\=1√x−1√x+1 

$\dfrac{d}{dx}\left(\arctanh\left(x\right)\right)=\dfrac{1}{1-x^2}$ddx (arctanh(x))\=11−x<sup class=""><span>2</span></sup>  $\dfrac{d}{dx}\left(\arcsech\left(x\right)\right)=\dfrac{\sqrt{\dfrac{2}{x+1}-1}}{\left(x-1\right)x}$ddx (arcsech(x))\=√2x+1 −1(x−1)x 

$\dfrac{d}{dx}\left(\arccsch\left(x\right)\right)=-\dfrac{1}{\sqrt{\dfrac{1}{x^2}+1}x^2}$ddx (arccsch(x))\=−1√1x<sup class=""><span>2</span></sup> +1x<sup class=""><span>2</span></sup>